theories/AAsynToSem.v
@@ -1,8 +1,7 @@
 (** Define translation from syntactic terms/values to semantic ones, following Sec. 3.2 of the PDF. *)
 From iris.proofmode Require Import tactics.
 From iris.program_logic Require Import ectx_lifting.
-From Dot Require Import tactics synFuncs operational synLemmas.
-Import operational.lang.
+From Dot Require Import tactics operational synLemmas.
 
 Section Sec.
   Context `{HdotG: dotG Σ}.
