theories/lr_lemma.v
@@ -22,8 +22,8 @@ Implicit Types e : expr Λ.
 
 End wp_extra.
 
-From iris.program_logic Require Import lifting language ectxi_language.
-From Dot Require Import tactics unary_lr rules synLemmas.
+From iris.program_logic Require Import lifting language.
+From Dot Require Import tactics rules synLemmas unary_lr_binding.
 Implicit Types (L T U: ty) (v: vl) (e: tm) (d: dm) (ds: dms) (Γ : ctx).
 Section Sec.
   Context `{HdotG: dotG Σ} Γ.
@@ -47,9 +47,9 @@ Section Sec.
     iApply (wp_wand_cl (e.|[to_subst ρ]) _ (⟦ T2 ⟧ ρ)).
     3: {iIntros; iApply "Hsub" => //. }
     iApply ("HeT1" $! ρ with "Hg").
-    iPoseProof (interp_env_len_agree with "Hg") as "%". move: H => Hlen.
     iPoseProof (interp_env_ρ_closed with "Hg") as "%". move: H => Hclρ.
-    iPureIntro. rewrite <- Hlen in Hcle. by apply fv_to_subst.
+    iPoseProof (interp_env_len_agree with "Hg") as "%". move: H => Hlen. rewrite <- Hlen in Hcle.
+    iPureIntro. by apply fv_to_subst.
   Qed.
 
   Lemma T_Var x T:
@@ -62,34 +62,6 @@ Section Sec.
     by iApply interp_env_lookup.
   Qed.
 
-  Lemma Sub_Refl T i : Γ ⊨ [T, i] <: [T, i].
-  Proof. by iIntros "/= !> **". Qed.
-
-  Lemma Sub_Trans T1 T2 T3 i1 i2 i3 : (Γ ⊨ [T1, i1] <: [T2, i2] →
-                                       Γ ⊨ [T2, i2] <: [T3, i3] →
-                                       Γ ⊨ [T1, i1] <: [T3, i3])%I.
-  Proof.
-    iIntros "#Hsub1 #Hsub2 /= !> * % #Hg #HT".
-    iApply "Hsub2" => //. by iApply "Hsub1".
-  Qed.
-
-  Lemma Sub_Mono e T i :
-    (Γ ⊨ [T, i] <: [T, S i])%I.
-  Proof. by iIntros "!> **". Qed.
-
-  Lemma Later_Sub e T i :
-    (Γ ⊨ [TLater T, i] <: [T, S i])%I.
-  Proof. by iIntros "/= !>" (ρ v Hclv) "#HG #[Hcl HT] !>". Qed.
-
-  Lemma Sub_Later e T i :
-    (Γ ⊨ [T, S i] <: [TLater T, i])%I.
-  Proof. iIntros "/= !> ** !>". naive_solver. Qed.
-
-  Lemma Sub_Index_Incr e T U i j:
-    (Γ ⊨ [T, i] <: [U, j] →
-     Γ ⊨ [T, S i] <: [U, S j])%I.
-  Proof. iIntros "/= #Hsub !> ** !>". by iApply "Hsub". Qed.
-
   Lemma T_Skip e T i:
     (Γ ⊨ e : T, S i →
      Γ ⊨ tskip e : T, i)%I.
@@ -98,47 +70,6 @@ Section Sec.
     iApply wp_pure_step_later; auto.
     iSpecialize ("HT" $! ρ with "HG"). by iModIntro.
   Qed.
-
-  Lemma And1_Sub T1 T2 i: Γ ⊨ [TAnd T1 T2, i] <: [T1, i].
-  Proof. by iIntros "/= !> * ? ? [? ?]". Qed.
-  Lemma And2_Sub T1 T2 i: Γ ⊨ [TAnd T1 T2, i] <: [T2, i].
-  Proof. by iIntros "/= !> * ? ? [? ?]". Qed.
-
-  (* Lemma stp_andi T1 T2 ρ v: *)
-  (*   ⟦T1⟧ ρ v -∗ *)
-  (*   ⟦T2⟧ ρ v -∗ *)
-  (*   ⟦TAnd T1 T2⟧ ρ v. *)
-  (* Proof. iIntros; by iSplit. Qed. *)
-
-  Lemma Sub_And S T1 T2 i j:
-    Γ ⊨ [S, i] <: [T1, j] -∗
-    Γ ⊨ [S, i] <: [T2, j] -∗
-    Γ ⊨ [S, i] <: [TAnd T1 T2, j].
-  Proof.
-    iIntros "/= #H1 #H2 !> * #Hcl #Hg #HS".
-    iSpecialize ("H1" with "Hcl Hg HS").
-    iSpecialize ("H2" with "Hcl Hg HS").
-    iModIntro; by iSplit.
-  Qed.
-
-  Lemma Sub_Or1 T1 T2 i: Γ ⊨ [T1, i] <: [TOr T1 T2, i].
-  Proof. iIntros "/= !> ** !>"; naive_solver. Qed.
-  Lemma Sub_Or2 T1 T2 i: Γ ⊨ [T2, i] <: [TOr T1 T2, i].
-  Proof. iIntros "/= !> ** !>"; naive_solver. Qed.
-
-  Lemma Or_Sub S T1 T2 i j:
-    Γ ⊨ [T1, i] <: [S, j] -∗
-    Γ ⊨ [T2, i] <: [S, j] -∗
-    Γ ⊨ [TOr T1 T2, i] <: [S, j].
-  Proof. iIntros "/= #H1 #H2 !> * #Hcl #Hg #[HT1 | HT2]"; by [iApply "H1" | iApply "H2"]. Qed.
-
-  Lemma Sub_Top T i:
-    Γ ⊨ [T, i] <: [TTop, i].
-  Proof. by iIntros "!> ** /=". Qed.
-
-  Lemma Bot_Sub T i:
-    Γ ⊨ [TBot, i] <: [T, i].
-  Proof. by iIntros "/= !> ** !>". Qed.
 
   (*
      Γ, z: T₁ᶻ ⊨ T₁ᶻ <: T₂ᶻ
@@ -225,12 +156,15 @@ Section Sec.
     iSplit; eauto using fv_tv, fv_vabs.
     iIntros " !> * #HG".
     iPoseProof (interp_env_ρ_closed with "HG") as "%". move: H => Hclρ.
-    iAssert (⌜ length ρ = length Γ ⌝)%I as "%". by iApply interp_env_len_agree. move: H => Hlen.
+    iPoseProof (interp_env_len_agree with "HG") as "%". move: H => Hlen. rewrite <- Hlen in Hcle.
+    (* iAssert (⌜ length ρ = length Γ ⌝)%I as "%". by iApply interp_env_len_agree. move: H => Hlen. *)
     iApply wp_value'.
     iSplit.
     { 
-      iPureIntro. rewrite <- Hlen in *.
-      pose proof (fv_to_subst (tv (vabs e)) ρ) as Hfv. asimpl in Hfv.
+      iPureIntro.
+      (* Applying the lemma directly fails due to the ordering of typeclass
+         search. Canonical structures would probably avoid that problem. *)
+      pose proof (fv_to_subst (tv (vabs e)) ρ) as Hfv.
       (* apply fv_tv_inv, Hfv => //; apply fv_tv, fv_vabs, Hcle. *)
       eauto using fv_tv_inv, fv_vabs, fv_tv.
     }
@@ -255,7 +189,7 @@ Section Sec.
     simplOpen ds; subst.
     match goal with H: _ @ _ ↘ _ |- _ => inversion H; ev; injectHyps end.
     iApply wp_pure_step_later; eauto.
-    by iApply wp_value'.
+    by iApply wp_value.
   Qed.
 
   (* BEWARE NONSENSE IN NOTES:
@@ -289,5 +223,6 @@ Section Sec.
     ivtp Γ (TMu T) v -∗
     ivtp Γ T.|[v/] v).
   Proof. by intros; iDestruct ivstp_rec_eq as "[? ?]". Qed.
+
 
 End Sec.
