theories/lr_lemma_nobinding.v
@@ -1,0 +1,79 @@
+From iris.base_logic Require Import base_logic.
+From iris.proofmode Require Import tactics.
+From Dot Require Import unary_lr.
+
+Implicit Types (L T U: ty) (v: vl) (e: tm) (d: dm) (ds: dms) (Γ : ctx).
+
+Section Sec.
+  Context `{HdotG: dotG Σ} Γ.
+
+  Lemma Sub_Refl T i : Γ ⊨ [T, i] <: [T, i].
+  Proof. by iIntros "/= !> **". Qed.
+
+  Lemma Sub_Trans T1 T2 T3 i1 i2 i3 : (Γ ⊨ [T1, i1] <: [T2, i2] →
+                                       Γ ⊨ [T2, i2] <: [T3, i3] →
+                                       Γ ⊨ [T1, i1] <: [T3, i3])%I.
+  Proof.
+    iIntros "#Hsub1 #Hsub2 /= !> * % #Hg #HT".
+    iApply "Hsub2" => //. by iApply "Hsub1".
+  Qed.
+
+  Lemma Sub_Mono e T i :
+    (Γ ⊨ [T, i] <: [T, S i])%I.
+  Proof. by iIntros "!> **". Qed.
+
+  Lemma Later_Sub e T i :
+    (Γ ⊨ [TLater T, i] <: [T, S i])%I.
+  Proof. by iIntros "/= !>" (ρ v Hclv) "#HG #[Hcl HT] !>". Qed.
+
+  Lemma Sub_Later e T i :
+    (Γ ⊨ [T, S i] <: [TLater T, i])%I.
+  Proof. iIntros "/= !> ** !>". naive_solver. Qed.
+
+  Lemma Sub_Index_Incr e T U i j:
+    (Γ ⊨ [T, i] <: [U, j] →
+     Γ ⊨ [T, S i] <: [U, S j])%I.
+  Proof. iIntros "/= #Hsub !> ** !>". by iApply "Hsub". Qed.
+
+  Lemma And1_Sub T1 T2 i: Γ ⊨ [TAnd T1 T2, i] <: [T1, i].
+  Proof. by iIntros "/= !> * ? ? [? ?]". Qed.
+  Lemma And2_Sub T1 T2 i: Γ ⊨ [TAnd T1 T2, i] <: [T2, i].
+  Proof. by iIntros "/= !> * ? ? [? ?]". Qed.
+
+  (* Lemma stp_andi T1 T2 ρ v: *)
+  (*   ⟦T1⟧ ρ v -∗ *)
+  (*   ⟦T2⟧ ρ v -∗ *)
+  (*   ⟦TAnd T1 T2⟧ ρ v. *)
+  (* Proof. iIntros; by iSplit. Qed. *)
+
+  Lemma Sub_And S T1 T2 i j:
+    Γ ⊨ [S, i] <: [T1, j] -∗
+    Γ ⊨ [S, i] <: [T2, j] -∗
+    Γ ⊨ [S, i] <: [TAnd T1 T2, j].
+  Proof.
+    iIntros "/= #H1 #H2 !> * #Hcl #Hg #HS".
+    iSpecialize ("H1" with "Hcl Hg HS").
+    iSpecialize ("H2" with "Hcl Hg HS").
+    iModIntro; by iSplit.
+  Qed.
+
+  Lemma Sub_Or1 T1 T2 i: Γ ⊨ [T1, i] <: [TOr T1 T2, i].
+  Proof. iIntros "/= !> ** !>"; naive_solver. Qed.
+  Lemma Sub_Or2 T1 T2 i: Γ ⊨ [T2, i] <: [TOr T1 T2, i].
+  Proof. iIntros "/= !> ** !>"; naive_solver. Qed.
+
+  Lemma Or_Sub S T1 T2 i j:
+    Γ ⊨ [T1, i] <: [S, j] -∗
+    Γ ⊨ [T2, i] <: [S, j] -∗
+    Γ ⊨ [TOr T1 T2, i] <: [S, j].
+  Proof. iIntros "/= #H1 #H2 !> * #Hcl #Hg #[HT1 | HT2]"; by [iApply "H1" | iApply "H2"]. Qed.
+
+  Lemma Sub_Top T i:
+    Γ ⊨ [T, i] <: [TTop, i].
+  Proof. by iIntros "!> ** /=". Qed.
+
+  Lemma Bot_Sub T i:
+    Γ ⊨ [TBot, i] <: [T, i].
+  Proof. by iIntros "/= !> ** !>". Qed.
+
+End Sec.
