theories/synLemmas.v
@@ -3,115 +3,7 @@ Lemmas on SynFuncs.v needed for proofs on the operational semantics.
 To reduce compile times, unary_lr should not depend on this file.
 This file should load as little Iris code as possible, to reduce compile times.
  *)
-From Dot Require Import tactics dotsyn synFuncs.
-
-(** Rewrite v ↗ ds to vobj ds' ↗ ds. *)
-Ltac simplOpen ds' :=
-  lazymatch goal with
-  | H: ?v @ ?l ↘ ?d |-_=>
-    inversion H as (ds & -> & _)
-  end.
-
-(** Determinacy of obj_opens_to. *)
-Lemma objLookupDet v l d1 d2: v @ l ↘ d1 -> v @ l ↘ d2 -> d1 = d2.
-Proof.
-  rewrite /objLookup; intros; ev; by subst; injectHyps; optFuncs_det.
-Qed.
-Ltac objLookupDet :=
-  lazymatch goal with
-  | H1: ?v @ ?l ↘ ?d1, H2: ?v @ ?l ↘ ?d2 |- _=>
-    assert (d2 = d1) as ? by (eapply objLookupDet; eassumption); injectHyps
-  end.
-
-(** Auxiliary definitions to prove [lookup_reverse_length], since a direct inductive proof appers to fail (but
-see rev_append_map for an approach that has a chance). *)
-Fixpoint indexr {X} (i: nat) (xs: list X) : option X :=
-  match xs with
-  | [] => None
-  | x :: xs =>
-    if decide (i = length xs) then Some x else indexr i xs
-  end.
-
-Lemma indexr_max {X} (T: X) i vs:
-                       indexr i vs = Some T ->
-                       i < length vs.
-Proof.
-  induction vs; first done; rewrite /lt in IHvs |- *; move => /= H.
-  case_decide; subst; [ lia | eauto ].
-Qed.
-Hint Resolve indexr_max.
-
-Lemma lookup_reverse_indexr {X} (ds: list X) l: reverse ds !! l = indexr l ds.
-Proof.
-  elim: ds l => [|d ds IHds] l //=.
-  case_decide; subst.
-  - rewrite reverse_cons lookup_app_r reverse_length ?Nat.sub_diag //=.
-  - case (decide (l < length ds)) => Hl.
-    + rewrite reverse_cons lookup_app_l ?reverse_length //=.
-    + assert (l > length ds) by omega.
-      assert (indexr l ds = None). {
-        destruct (indexr l ds) eqn:? => //.
-        assert (l < length ds) by (eapply indexr_max; eauto); lia.
-      }
-      rewrite lookup_ge_None_2 ?reverse_length //=.
-Qed.
-
-Lemma lookup_reverse_length {X} l (d: X) ds: l = length ds → reverse (d :: ds) !! l = Some d.
-Proof.
-  intros; subst. rewrite lookup_reverse_indexr /=. case_decide => //=.
-Qed.
-
-Lemma obj_lookup_cons d ds: vobj (d :: ds) @ length ds ↘ d.|[vobj (d :: ds)/].
-Proof.
-  hnf. eexists; split; trivial.
-  rewrite /selfSubst /=. apply lookup_reverse_length. by rewrite map_length.
-Qed.
-
-Lemma indexr_extend {X} vs n x (T: X):
-                       indexr n vs = Some T ->
-                       indexr n (x::vs) = Some T.
-Proof.
-  move => H /=; assert (n < length vs) by naive_solver; by case_decide; first lia.
-Qed.
-Hint Resolve indexr_extend.
-
-Lemma lookup_reverse_extend {X} l (d: X) ds:
-  reverse ds !! l = Some d →
-  reverse (d :: ds) !! l = Some d.
-Proof.
-  intros; subst. rewrite -> lookup_reverse_indexr in *. by apply indexr_extend.
-Qed.
-
-Lemma rev_append_map {X Y} (xs1 xs2: list X) (f: X → Y): rev_append (map f xs1) (map f xs2) = map f (rev_append xs1 xs2).
-Proof.
-  elim: xs1 xs2 => [|x xs1 IH] xs2 //=. eapply (IH (x :: xs2)).
-Qed.
-Lemma reverse_map {X Y} (xs: list X) (f: X → Y): reverse (map f xs) = map f (reverse xs).
-Proof. rewrite /reverse. eapply (rev_append_map xs []). Qed.
-
-Lemma lookup_map {X Y} x (xs: list X) (f: X → Y) l: xs !! l = Some x → map f xs !! l = Some (f x).
-Proof.
-  elim: xs l => /= [|x' xs IH] [|l] //= Hl; by [cinject Hl | apply IH].
-Qed.
-
-(* Lemma lookup_map_inv {X Y} x (xs: list X) (f: X → Y) l: map f xs !! l = Some (f x) → xs !! l = Some x. *)
-(* Proof. *)
-(*   elim: xs l => [|x' xs IH] [|l] //=. (* ONLY FOR F INDUCTIVE! *) *)
-
-(* Lemma obj_lookup_extend d ds l: *)
-(*   vobj ds @ l ↘ d.|[vobj ds/] → *)
-(*   vobj (d :: ds) @ l ↘ d.|[vobj (d :: ds)/]. *)
-(* Proof. *)
-(*   hnf. *)
-(*   intros (ds0 & Heq & Hl). cinject Heq. *)
-(*   eexists; split; trivial. *)
-(*   move: Hl. rewrite /selfSubst /lookup_reverse_indexr /= => Hl. *)
-(*   apply lookup_reverse_extend. *)
-(*   move: Hl. rewrite /hsubst /HSubst_dm !reverse_map => Hl. *)
-(*   apply lookup_map. apply lookup_map_inv in Hl. apply Hl. *)
-(*   (* eauto using lookup_map, lookup_map_inv. *) *)
-(* Qed. *)
-
+From Dot Require Import tactics dotsyn.
 
 (* Auxiliary lemma for [length_idsσ]. *)
 Lemma length_idsσr n r: length (idsσ n).|[ren r] = n.
@@ -171,6 +63,7 @@ Proof.
 Qed.
 
 Lemma closed_to_subst ρ x: cl_ρ ρ → x < length ρ → nclosed_vl (to_subst ρ x) 0.
+Proof.
   elim: ρ x => /= [|v ρ IHρ] [|x] Hcl Hl; asimpl; try omega; inverse Hcl; try by [].
   by apply IHρ; try omega.
 Qed.
