theories/unary_lr.v
@@ -1,6 +1,6 @@
 From iris.program_logic Require Import weakestpre.
 From iris.proofmode Require Import tactics.
-From Dot Require Export operational tactics synLemmas.
+From Dot Require Export operational tactics.
 
 (** Deduce types from variable names, like on paper, for readability and to help
     type inference for some overloaded operations (e.g. substitution). *)
@@ -158,22 +158,6 @@ Section logrel.
     Persistent (def_interp T l ρ d).
   Proof. revert ρ d; induction T; simpl; try apply _. Qed.
 
-  Lemma interp_v_closed T v ρ: (interp T ρ v → ⌜ nclosed_vl v 0 ⌝)%I.
-  Proof.
-    iInduction T as [] "IHT" forall (ρ v); iIntros "#HT //="; try by iDestruct "HT" as "[% _]".
-    (* move: ρ v; induction T; iIntros (ρ v) "HT //="; try solve [by iDestruct "HT" as "[% _]"]. *)
-    - iDestruct "HT" as "[#HT1 #HT2]". by iApply "IHT".
-    - iDestruct "HT" as "[#HT1 | #HT2]"; by [iApply "IHT" | iApply "IHT1"].
-    - by iApply "IHT".
-    - iDestruct "HT" as "[#HT2 _]". by iApply "IHT1".
-    - iDestruct "HT" as (n) "%"; subst. iPureIntro. solve_fv_congruence.
-  Qed.
-
-  Lemma def_interp_v_closed T d l ρ: (def_interp T l ρ d → ⌜ nclosed d 0 ⌝)%I.
-  Proof.
-    iInduction T as [] "IH" forall (ρ d); iIntros "#HT //="; by iDestruct "HT" as "[% [% _]]".
-  Qed.
-
   Program Definition defs_interp_and
              (interp1 : listVlC -n> dmsC -n> iProp Σ)
              (interp2: label -> listVlC -n> dmC -n> iProp Σ)
@@ -195,16 +179,6 @@ Section logrel.
     Persistent (defs_interp T ρ ds).
   Proof.
     revert ds ρ; induction T; simpl; intros; try case_match; try apply _.
-  Qed.
-
-  Lemma defs_interp_v_closed T ds ρ: (defs_interp T ρ ds → ⌜ nclosed ds 0 ⌝)%I.
-  Proof.
-    iInduction T as [] "IH" forall (ρ ds); iIntros "#HT //=".
-    destruct ds. done.
-    iDestruct "HT" as "[HT1 HT2]".
-    iPoseProof ("IH" with "HT1") as "%".
-    iPoseProof (def_interp_v_closed with "HT2") as "%".
-    iPureIntro. by apply fv_dms_cons.
   Qed.
 
   Fixpoint interp_env (Γ : ctx) (vs : vls) : iProp Σ :=
@@ -300,7 +274,6 @@ Notation "Γ ⊨ e : T , i" := (step_indexed_ietp Γ T e i) (at level 74, e, T a
 Notation "Γ ⊨ T1 <: T2" := (ivstp Γ T1 T2) (at level 74, T1, T2 at next level).
 Notation "Γ '⊨' '[' T1 ',' i ']' '<:' '[' T2 ',' j ']'" := (step_indexed_ivstp Γ T1 T2 i j) (at level 74, T1, T2 at next level).
 
-(* Lemmas about the logical relation itself. *)
 Section logrel_lemmas.
   Context `{HdotG: dotG Σ}.
 
@@ -312,35 +285,6 @@ Section logrel_lemmas.
     iSplit; by [iIntros "#[_ $]" | iIntros "$"].
   Qed.
 
-  Lemma interp_weaken ρ1 ρ2 ρ3 τ :
-    ⟦ τ.|[upn (length ρ1) (ren (+ length ρ2))] ⟧ (ρ1 ++ ρ2 ++ ρ3)
-    ≡ ⟦ τ ⟧ (ρ1 ++ ρ3).
-  Proof.
-    revert ρ1 ρ2 ρ3; induction τ=> ρ1 ρ2 ρ3 w; simpl; trivial; asimpl;
-                                    rewrite ?to_subst_weaken.
-    all: try solve [properness; trivial;
-                    apply IHτ || apply IHτ1 || apply IHτ2 ||
-                          apply (IHτ2 (_ :: _)) || apply (IHτ (_ :: _))].
-  Qed.
-
-  Lemma interp_weaken_one v τ ρ:
-     ⟦ τ.|[ren (+1)] ⟧ (v :: ρ) ≡ ⟦ τ ⟧ ρ.
-  Proof. apply (interp_weaken [] [v]). Qed.
-
-  Lemma interp_subst_up ρ1 ρ2 τ v:
-    ⟦ τ.|[upn (length ρ1) (v.[ren (+length ρ2)] .: ids)] ⟧ (ρ1 ++ ρ2)
-    ≡ ⟦ τ ⟧ (ρ1 ++ v :: ρ2).
-  Proof.
-    revert ρ1 ρ2; induction τ=> ρ1 ρ2 w; simpl; trivial; asimpl;
-                                    rewrite ?to_subst_up.
-    all: try solve [properness; trivial;
-                    apply IHτ || apply IHτ1 || apply IHτ2 ||
-                          apply (IHτ2 (_ :: _)) || apply (IHτ (_ :: _))].
-  Qed.
-
-  Lemma interp_subst ρ τ v1 v2 : ⟦ τ.|[v1.[ren (+length ρ)]/] ⟧ ρ v2 ≡ ⟦ τ ⟧ (v1 :: ρ) v2.
-  Proof. apply (interp_subst_up []). Qed.
-
   Context Γ.
 
   Lemma semantic_typing_uniform_step_index T e i:
@@ -350,19 +294,15 @@ Section logrel_lemmas.
     iInduction i as [|i] "IHi". by iApply "H". iApply "IHi".
   Qed.
 
-  Lemma interp_env_lookup ρ T x:
-    Γ !! x = Some T →
-    (⟦ Γ ⟧* ρ → ⟦ T.|[ren (+x)] ⟧ ρ (to_subst ρ x))%I.
+  Lemma interp_v_closed T v ρ: (interp T ρ v → ⌜ nclosed_vl v 0 ⌝)%I.
   Proof.
-    iIntros (Hx) "* #Hg".
-    iInduction Γ as [|T' Γ'] "IHL" forall (x ρ Hx); simpl; try solve [inversion Hx].
-    destruct ρ; try by iExFalso.
-    iDestruct "Hg" as "[̋Hg Ht]".
-    case: x Hx => /= [|x] Hx.
-    - move: Hx => [ -> ]. iSpecialize ("IHL" $! 0). by asimpl.
-    - rewrite to_subst_cons /=.
-      iAssert (⟦ T.|[ren (+x)] ⟧ ρ (to_subst ρ x)) as "#Hv". by iApply "IHL".
-      iPoseProof (interp_weaken [] [v] ρ with "Hv") as "H"; asimpl. iExact "H".
+    iInduction T as [] "IHT" forall (ρ v); iIntros "#HT //="; try by (iDestruct "HT" as "[% _]").
+    (* move: ρ v; induction T; iIntros (ρ v) "HT //="; try solve [by iDestruct "HT" as "[% _]"]. *)
+    - iDestruct "HT" as "[#HT1 #HT2]". by iApply "IHT".
+    - iDestruct "HT" as "[#HT1 | #HT2]"; by [iApply "IHT" | iApply "IHT1"].
+    - by iApply "IHT".
+    - iDestruct "HT" as "[#HT2 _]". by iApply "IHT1".
+    - by iDestruct "HT" as (n) "->".
   Qed.
 
   Lemma interp_env_len_agree ρ:
@@ -370,32 +310,8 @@ Section logrel_lemmas.
   Proof.
     iInduction Γ as [|τ Γ'] "IHΓ" forall (ρ); destruct ρ => //=.
     iIntros "#[HG Hv]".
-    Fail iRewrite ("IHΓ" $! ρ with "HG").
+    (* Fail iRewrite ("IHΓ" $! ρ with "HG"). *)
     by iDestruct ("IHΓ" $! ρ with "HG") as "->".
-  Qed.
-
-  Lemma interp_subst_all ρ τ v:
-    cl_ρ ρ → ⟦ τ.|[to_subst ρ] ⟧ [] v ≡ ⟦ τ ⟧ ρ v.
-  Proof.
-    elim: ρ τ => /= [|w ρ IHρ] τ Hwρcl; asimpl; first by [].
-    assert (nclosed_vl w 0 /\ Forall (λ v, nclosed_vl v 0) ρ) as [Hwcl Hρcl]. by inversion Hwρcl.
-    specialize (IHρ (τ.|[w/]) Hρcl).
-    asimpl in IHρ. move: IHρ. rewrite closed_subst_vl_id// => IHρ.
-    rewrite IHρ -interp_subst closed_subst_vl_id //.
-  Qed.
-
-  Lemma to_subst_interp T ρ v w: cl_ρ ρ → nclosed_vl v (length ρ) →
-    ⟦ T.|[v/] ⟧ ρ w ≡ ⟦ T.|[v.[to_subst ρ]/] ⟧ ρ w.
-  Proof.
-    intros Hclρ Hclv.
-    assert (v.[to_subst ρ] = v.[to_subst ρ >> to_subst ρ]) as Hrew. {
-      apply Hclv.
-      intros x Hl.
-      asimpl.
-      rewrite closed_subst_vl_id //. by apply closed_to_subst.
-    }
-    rewrite -(interp_subst_all ρ (T.|[v/])) // -(interp_subst_all ρ (T.|[v.[to_subst ρ]/])) //.
-    asimpl. by rewrite -Hrew.
   Qed.
 
   Lemma interp_env_ρ_closed ρ: (⟦ Γ ⟧* ρ → ⌜ cl_ρ ρ ⌝)%I.
@@ -405,67 +321,6 @@ Section logrel_lemmas.
     iPoseProof (interp_v_closed with "HT") as "%".
     iPoseProof (IHl with "HG") as "%".
     iPureIntro; by constructor.
-  Qed.
-
-  Lemma interp_env_to_subst_closed ρ x: x < length ρ → (⟦ Γ ⟧* ρ → ⌜ nclosed_vl (to_subst ρ x) 0 ⌝)%I.
-  Proof.
-    iIntros (Hl) "#HG". iPoseProof (interp_env_ρ_closed with "HG") as "%".
-    iPureIntro; by apply closed_to_subst.
-  Qed.
-
-  Lemma ietp_closed_vl T v: (Γ ⊨ tv v : T → ⌜ nclosed_vl v (length Γ) ⌝)%I.
-  Proof.
-    iIntros "H".
-    iPoseProof (ietp_closed with "H") as "%". by iPureIntro; apply fv_tv_inv.
-  Qed.
-
-  (* Lemma interp_env_to_subst_closed ρ x: x < length ρ → (⟦ Γ ⟧* ρ → ⌜ nclosed_vl (to_subst ρ x) 0 ⌝)%I. *)
-  (* Proof. *)
-  (*   (* Hint Resolve defs_interp_v_closed def_interp_v_closed interp_v_closed. *) *)
-  (*   revert Γ ρ x. *)
-  (*   elim => [|T Γ IHl] [|v ρ] [|x] /= Hl; try omega; try (iIntros "%"; discriminate); iIntros "[#HG #HT]". *)
-  (*   - iApply interp_v_closed. rewrite to_subst_cons /=. iApply "HT". *)
-  (*   - asimpl. by iApply IHl; first omega. *)
-  (* Qed. *)
-
-  (* Lemma interp_subst_closed T v w ρ: *)
-  (*   nclosed_vl v (length ρ) → *)
-  (*   (⟦ Γ ⟧* ρ → ⟦ T.|[v/] ⟧ ρ w ∗-∗ ⟦ T ⟧ (v.[to_subst ρ] :: ρ) w)%I. *)
-  (* Proof. *)
-  (*   iIntros (Hcl) "#HG". *)
-  (*   iAssert ⌜ cl_ρ ρ ⌝%I as "%". by iApply interp_env_ρ_closed. move: H => Hclρ. *)
-  (*   assert (⟦ T.|[v.[to_subst ρ]/] ⟧ ρ w ≡ ⟦ T.|[v/] ⟧ ρ w) as Hren. by rewrite (to_subst_interp T ρ v w). *)
-  (*   iPoseProof (interp_subst ρ T (v.[to_subst ρ]) w) as "Heq"; asimpl. *)
-  (*   iAssert (⌜ eq_n_s (to_subst ρ >> ren (+length ρ)) (to_subst ρ) (length ρ) ⌝)%I as "%". *)
-  (*   { *)
-  (*     iIntros (x Hxl). *)
-  (*     iPoseProof (interp_env_to_subst_closed ρ x Hxl with "HG") as "%". move: H => Hclx. *)
-  (*     iPureIntro; apply closed_subst_vl_id, Hclx. *)
-  (*   } *)
-  (*   rewrite (Hcl (to_subst ρ >> ren (+length ρ)) (to_subst ρ)) //. *)
-  (*   rewrite Hren. *)
-  (*   iExact "Heq". *)
-  (* Qed. *)
-
-  (* Try giving a simpler proof: *)
-  Lemma interp_subst_closed_aux T v w ρ:
-    nclosed_vl v (length ρ) →
-    (⟦ Γ ⟧* ρ → ⟦ T.|[v/] ⟧ ρ w ∗-∗ ⟦ T ⟧ (v.[to_subst ρ] :: ρ) w)%I.
-  Proof.
-    iIntros (Hcl) "#Hg".
-    iPoseProof (interp_env_ρ_closed ρ with "Hg") as "%"; move: H => Hclρ.
-    iPoseProof (interp_subst ρ T (v.[to_subst ρ]) w) as "Heq"; iEval (asimpl) in "Heq".
-    rewrite (Hcl (to_subst ρ >> ren (+length ρ)) (to_subst ρ)) // -?(to_subst_interp T ρ v w) //.
-    move => x Hlρ. asimpl. by rewrite closed_subst_vl_id; [|apply closed_to_subst].
-  Qed.
-
-  Lemma interp_subst_closed T v w ρ:
-    nclosed_vl v (length Γ) →
-    (⟦ Γ ⟧* ρ → ⟦ T.|[v/] ⟧ ρ w ∗-∗ ⟦ T ⟧ (v.[to_subst ρ] :: ρ) w)%I.
-  Proof.
-    iIntros (Hcl) "#Hg".
-    iPoseProof (interp_env_len_agree ρ with "Hg") as "%"; move: H => HlenEq; rewrite <- HlenEq in *.
-    by iApply interp_subst_closed_aux.
   Qed.
 
 End logrel_lemmas.
